instantiation/SystemRegisterAccess.thy
@@ -19,13 +19,13 @@ begin
 section \<open>System register access\<close>
 
 lemma NumberedRegisterIsAccessible:
-  assumes reg: "cd \<in> \<Union> (CapDerivationRegisters ` actions)"
+  assumes reg: "cd \<in> \<Union> (SpecialRegisterParameters ` actions)"
       and valid: "getStateIsValid s"
       and suc: "(PreserveDomain actions, s') \<in> NextStates s"
   shows "getSpecial_register_accessible cd s"
 proof -
   obtain ac where ac: "ac \<in> actions"
-              and cd: "cd \<in> CapDerivationRegisters ac"
+              and cd: "cd \<in> SpecialRegisterParameters ac"
     using reg
     by auto
   have ghost: "getGhostStateIsValid s"
@@ -96,14 +96,14 @@ corollary SystemRegisterInstantiation:
 unfolding SystemRegisterProp_def
 proof clarify
   fix actions action cd
-  assume reg: "cd \<in> CapDerivationRegisters action"
+  assume reg: "cd \<in> SpecialRegisterParameters action"
      and action: "action \<in> actions"
      and system: "cd \<noteq> 0" "cd \<noteq> 1"
      and valid: "getStateIsValid s"
      and lbl: "lbl = PreserveDomain actions"
   have suc: "(PreserveDomain actions, s') \<in> NextStates s"
     using assms lbl by auto
-  have "cd \<in> \<Union> (CapDerivationRegisters ` actions)"
+  have "cd \<in> \<Union> (SpecialRegisterParameters ` actions)"
     using reg action by auto
   from NumberedRegisterIsAccessible[OF this valid suc]
   show "Access_System_Registers (getPerms (getPCC s))"
